LRATCatcher/Examples/Schur4CC/Base.lean
@@ -1,0 +1,20 @@
+import LRATCatcher.Cover
+import LRATCatcher.Showcases.Schur
+
+open Std.Sat LRATCatcher
+
+namespace LRATCatcher.Examples.Schur4CC
+
+def base : CNF Nat := LRATCatcher.Schur.encodeK 4 45
+
+def cubes : List Cube := LRATCatcher.parseICnf "a 1 2 3 0
+a 1 2 -3 0
+a 1 -2 3 0
+a 1 -2 -3 0
+a -1 2 3 0
+a -1 2 -3 0
+a -1 -2 3 0
+a -1 -2 -3 0
+"
+
+end LRATCatcher.Examples.Schur4CC
