LRATCatcher/Examples/Schur4CC/Cover.lean
@@ -1,0 +1,19 @@
+import LRATCatcher.Examples.Schur4CC.Base
+
+open Std.Sat LRATCatcher
+
+namespace LRATCatcher.Examples.Schur4CC
+
+set_option maxHeartbeats 0 in
+theorem coverThm : (negCubesCNF cubes).Unsat :=
+  LRATCatcher.checkLratCnf_sound _ "9 2 -1 0 4 3 0
+10 2 1 0 7 8 0
+11 -2 -1 0 1 2 0
+12 -2 1 0 6 5 0
+13 -1 0 9 11 0
+14 1 0 10 12 0
+15 1 0 14 0
+16 0 15 13 0
+" (by native_decide)
+
+end LRATCatcher.Examples.Schur4CC
